VisualProof.lean
@@ -43,5 +43,6 @@ import VisualProof.Rule.WirePrimitive.Content
 import VisualProof.Rule.WirePrimitive.ContentFixtures
 import VisualProof.Rule.WirePrimitive.ArgumentsFixtures
 import VisualProof.Rule.WirePrimitive.LeavesFixtures
+import VisualProof.Rule.WirePrimitive.CompilerFixtures
 import VisualProof.Rule.MonolithicWireQuantifier
 import VisualProof.Rule.MonolithicWireQuantifierFixtures
